@prefix dc: <http://purl.org/dc/elements/1.1/> .
@prefix dct: <http://purl.org/dc/terms/> .
@prefix owl: <http://www.w3.org/2002/07/owl#> .
@prefix rdfs: <http://www.w3.org/2000/01/rdf-schema#> .
@prefix skos: <http://www.w3.org/2004/02/skos/core#> .
@prefix xsd: <http://www.w3.org/2001/XMLSchema#> .

<https://vocabs.acdh.oeaw.ac.at/dha-taxonomy#collection1> a skos:Collection ;
    dc:creator "ACDH" ;
    dc:source "some sources"@en ;
    dct:created "2019-03-21T16:59:37.656139+00:00"^^xsd:dateTime ;
    dct:modified "2019-04-12T14:03:11.900910+00:00"^^xsd:dateTime ;
    skos:member <https://vocabs.acdh.oeaw.ac.at/dha-taxonomy#concept1>,
        <https://vocabs.acdh.oeaw.ac.at/dha-taxonomy#concept17>,
        <https://vocabs.acdh.oeaw.ac.at/dha-taxonomy#concept2>,
        <https://vocabs.acdh.oeaw.ac.at/dha-taxonomy#concept3>,
        <https://vocabs.acdh.oeaw.ac.at/dha-taxonomy#concept31>,
        <https://vocabs.acdh.oeaw.ac.at/dha-taxonomy#concept32>,
        <https://vocabs.acdh.oeaw.ac.at/dha-taxonomy#concept4>,
        <https://vocabs.acdh.oeaw.ac.at/dha-taxonomy#concept5> ;
    skos:prefLabel "Formats, Protocols, Standards"@en ;
    skos:scopeNote "This group comprises the concepts related to Formats, Protocols and Standards accepted and used in Digital Humanities community."@en .

<https://vocabs.acdh.oeaw.ac.at/dha-taxonomy#collection2> a skos:Collection ;
    dct:created "2019-04-10T15:35:07.115678+00:00"^^xsd:dateTime ;
    dct:modified "2019-04-10T15:35:07.166746+00:00"^^xsd:dateTime ;
    skos:member <https://vocabs.acdh.oeaw.ac.at/dha-taxonomy#concept23>,
        <https://vocabs.acdh.oeaw.ac.at/dha-taxonomy#concept26>,
        <https://vocabs.acdh.oeaw.ac.at/dha-taxonomy#concept27>,
        <https://vocabs.acdh.oeaw.ac.at/dha-taxonomy#concept28>,
        <https://vocabs.acdh.oeaw.ac.at/dha-taxonomy#concept29>,
        <https://vocabs.acdh.oeaw.ac.at/dha-taxonomy#concept30> ;
    skos:prefLabel "Resources"@en .

<https://vocabs.acdh.oeaw.ac.at/dha-taxonomy#collection3> a skos:Collection ;
    dc:creator "ACDH-OEAW Team" ;
    dct:created "2019-04-12T15:38:40.134646+00:00"^^xsd:dateTime ;
    dct:modified "2019-04-12T15:38:40.227677+00:00"^^xsd:dateTime ;
    skos:member <https://vocabs.acdh.oeaw.ac.at/dha-taxonomy#concept24>,
        <https://vocabs.acdh.oeaw.ac.at/dha-taxonomy#concept25> ;
    skos:prefLabel "Disciplines"@en ;
    skos:scopeNote "This group comprises the disciplines that are part of digital humanities research."@en .

<https://vocabs.acdh.oeaw.ac.at/dha-taxonomy#collection4> a skos:Collection ;
    dc:creator "ACDH-OEAW Team" ;
    dct:created "2019-04-12T15:39:40.156688+00:00"^^xsd:dateTime ;
    dct:modified "2019-04-12T15:39:40.221319+00:00"^^xsd:dateTime ;
    skos:member <https://vocabs.acdh.oeaw.ac.at/dha-taxonomy#concept33>,
        <https://vocabs.acdh.oeaw.ac.at/dha-taxonomy#concept34>,
        <https://vocabs.acdh.oeaw.ac.at/dha-taxonomy#concept35>,
        <https://vocabs.acdh.oeaw.ac.at/dha-taxonomy#concept36> ;
    skos:prefLabel "Tools and Services"@en ;
    skos:scopeNote "This group comprises the tool and services used in digital humanities field."@en .

<https://vocabs.acdh.oeaw.ac.at/dha-taxonomy#collection5> a skos:Collection ;
    dc:creator "ACDH-OEAW Team" ;
    dct:created "2019-04-12T15:40:17.551431+00:00"^^xsd:dateTime ;
    dct:modified "2019-04-12T15:40:17.630310+00:00"^^xsd:dateTime ;
    skos:member <https://vocabs.acdh.oeaw.ac.at/dha-taxonomy#concept20> ;
    skos:prefLabel "Topics"@en ;
    skos:scopeNote "This group comprises topics of research, discussion and application within digital humanities community."@en .

<https://vocabs.acdh.oeaw.ac.at/dha-taxonomy#concept21> a skos:Concept ;
    dct:created "2019-04-12T12:44:02.088801+00:00"^^xsd:dateTime ;
    dct:modified "2019-05-06T12:24:49.909633+00:00"^^xsd:dateTime ;
    skos:inScheme <https://vocabs.acdh.oeaw.ac.at/dha-taxonomy> ;
    skos:notation "activities" ;
    skos:prefLabel "Aktivitäten"@de,
        "activities"@en ;
    skos:topConceptOf <https://vocabs.acdh.oeaw.ac.at/dha-taxonomy> .

<https://vocabs.acdh.oeaw.ac.at/dha-taxonomy#concept17> a skos:Concept ;
    dc:source "\"TEI: Text Encoding Initiative.\" TEI: Text Encoding Initiative. Accessed June 13, 2016. http://www.tei-c.org/index.xml."@en ;
    dct:created "2019-04-10T14:56:24.117128+00:00"^^xsd:dateTime ;
    dct:modified "2019-05-06T12:30:15.784689+00:00"^^xsd:dateTime ;
    skos:altLabel "Text Encoding Initiative"@en ;
    skos:broader <https://vocabs.acdh.oeaw.ac.at/dha-taxonomy#concept31> ;
    skos:definition "a set of guidelines which specify encoding methods for machine-readable texts, chiefly in the humanities, social sciences and linguistics"@en ;
    skos:inScheme <https://vocabs.acdh.oeaw.ac.at/dha-taxonomy> ;
    skos:notation "tei" ;
    skos:prefLabel "TEI"@de,
        "TEI"@en ;
    skos:related <http://d-nb.info/gnd/5564213-5>,
        <http://dbpedia.org/resource/Text_Encoding_Initiative> .

<https://vocabs.acdh.oeaw.ac.at/dha-taxonomy#concept2> a skos:Concept ;
    dc:source "based on \"The CIDOC CRM.\" The CIDOC CRM. Accessed June 13, 2016. http://www.cidoc-crm.org/."@en ;
    dct:created "2019-03-21T17:07:48.239560+00:00"^^xsd:dateTime ;
    dct:modified "2019-05-06T12:28:57.694628+00:00"^^xsd:dateTime ;
    skos:altLabel "Comité international pour la documentation: Conceptual Reference Model"@fr ;
    skos:broader <https://vocabs.acdh.oeaw.ac.at/dha-taxonomy#concept1> ;
    skos:definition "a machine-readable ontology that provides definitions and a formal structure for describing general (top-level) concepts and relationships; used mainly in cultural heritage domain"@en ;
    skos:exactMatch <http://d-nb.info/gnd/1073990826> ;
    skos:inScheme <https://vocabs.acdh.oeaw.ac.at/dha-taxonomy> ;
    skos:notation "cidoc-crm" ;
    skos:prefLabel "CIDOC CRM"@de,
        "CIDOC CRM"@en .

<https://vocabs.acdh.oeaw.ac.at/dha-taxonomy#concept20> a skos:Concept ;
    dc:creator "ACDH-OEAW Team" ;
    dct:created "2019-04-11T09:47:05.237333+00:00"^^xsd:dateTime ;
    dct:modified "2019-05-06T12:25:43.498550+00:00"^^xsd:dateTime ;
    skos:definition "information about rights and conditions of use and distribution of resources"@en ;
    skos:inScheme <https://vocabs.acdh.oeaw.ac.at/dha-taxonomy> ;
    skos:notation "copyrights" ;
    skos:prefLabel "Urheberrecht und Lizenzierung"@de,
        "copyright and licensing"@en ;
    skos:related <http://d-nb.info/gnd/10286403-2>,
        <http://dbpedia.org/resource/Copyright> ;
    skos:topConceptOf <https://vocabs.acdh.oeaw.ac.at/dha-taxonomy> .

<https://vocabs.acdh.oeaw.ac.at/dha-taxonomy#concept24> a skos:Concept ;
    dc:source "archaeology. Oxford Dictionaries. Oxford University Press. http://www.oxforddictionaries.com/definition/english/archaeology (accessed February 28, 2016)."@en ;
    dct:created "2019-04-12T15:41:44.232803+00:00"^^xsd:dateTime ;
    dct:modified "2019-05-06T12:25:07.139284+00:00"^^xsd:dateTime ;
    skos:definition "the study of human history and prehistory through the excavation of sites and the analysis of artefacts and other physical remains"@en ;
    skos:inScheme <https://vocabs.acdh.oeaw.ac.at/dha-taxonomy> ;
    skos:notation "archaeology" ;
    skos:prefLabel "Archäologie"@de,
        "archaeology"@en ;
    skos:related <http://dbpedia.org/resource/Archaeology>,
        <http://www.eionet.europa.eu/gemet/concept/530> ;
    skos:topConceptOf <https://vocabs.acdh.oeaw.ac.at/dha-taxonomy> .

<https://vocabs.acdh.oeaw.ac.at/dha-taxonomy#concept25> a skos:Concept ;
    dc:source "Wikipedia contributors, \"Architecture,\" Wikipedia, The Free Encyclopedia, https://en.wikipedia.org/w/index.php?title=Architecture&oldid=712664162 (accessed April 4, 2016)."@en ;
    dct:created "2019-04-12T15:42:36.210028+00:00"^^xsd:dateTime ;
    dct:modified "2019-05-06T12:25:25.749907+00:00"^^xsd:dateTime ;
    skos:definition "both the process and the product of planning, designing, and constructing buildings and other physical structures"@en ;
    skos:inScheme <https://vocabs.acdh.oeaw.ac.at/dha-taxonomy> ;
    skos:notation "architecture" ;
    skos:prefLabel "Architektur"@de,
        "architecture"@en ;
    skos:related <http://dbpedia.org/resource/Architecture> ;
    skos:topConceptOf <https://vocabs.acdh.oeaw.ac.at/dha-taxonomy> .

<https://vocabs.acdh.oeaw.ac.at/dha-taxonomy#concept26> a skos:Concept ;
    dc:source "Wikipedia contributors, \"Text corpus,\" Wikipedia, The Free Encyclopedia, https://en.wikipedia.org/w/index.php?title=Text_corpus&oldid=701487841(accessed February 28, 2016)."@en ;
    dct:created "2019-04-12T15:50:53.834258+00:00"^^xsd:dateTime ;
    dct:modified "2019-05-06T12:26:16.957551+00:00"^^xsd:dateTime ;
    skos:broader <https://vocabs.acdh.oeaw.ac.at/dha-taxonomy#concept23> ;
    skos:definition "a large and structured set of texts electronically stored and processed"@en ;
    skos:inScheme <https://vocabs.acdh.oeaw.ac.at/dha-taxonomy> ;
    skos:notation "corpus-1" ;
    skos:prefLabel "Korpus"@de,
        "corpus"@en ;
    skos:related <http://d-nb.info/gnd/7671571-1> .

<https://vocabs.acdh.oeaw.ac.at/dha-taxonomy#concept27> a skos:Concept ;
    dc:source "Wikipedia contributors, \"Historical language,\" Wikipedia, The Free Encyclopedia, https://en.wikipedia.org/w/index.php?title=Historical_language&oldid=688305297 (accessed February 8, 2018)."@en ;
    dct:created "2019-04-12T15:52:00.949727+00:00"^^xsd:dateTime ;
    dct:modified "2019-05-06T12:26:33.780039+00:00"^^xsd:dateTime ;
    skos:broader <https://vocabs.acdh.oeaw.ac.at/dha-taxonomy#concept23> ;
    skos:definition "a language that is spoken in a historical period, but that is distinct from its modern form; that is, it is a form of language historically attested to from the past which has evolved into more modern forms"@en ;
    skos:inScheme <https://vocabs.acdh.oeaw.ac.at/dha-taxonomy> ;
    skos:notation "historical-language" ;
    skos:prefLabel "historische Sprache"@de,
        "historical language"@en .

<https://vocabs.acdh.oeaw.ac.at/dha-taxonomy#concept28> a skos:Concept ;
    dc:creator "ACDH-OEAW Team" ;
    dct:created "2019-04-12T15:53:30.102220+00:00"^^xsd:dateTime ;
    dct:modified "2019-05-06T12:26:49.389569+00:00"^^xsd:dateTime ;
    skos:broader <https://vocabs.acdh.oeaw.ac.at/dha-taxonomy#concept23> ;
    skos:definition "any text created in the past"@en ;
    skos:inScheme <https://vocabs.acdh.oeaw.ac.at/dha-taxonomy> ;
    skos:notation "historical-text" ;
    skos:prefLabel "historischer Text"@de,
        "historical text"@en .

<https://vocabs.acdh.oeaw.ac.at/dha-taxonomy#concept29> a skos:Concept ;
    dc:creator "ACDH-OEAW Team" ;
    dct:created "2019-04-12T15:54:15.862852+00:00"^^xsd:dateTime ;
    dct:modified "2019-05-06T12:27:07.662824+00:00"^^xsd:dateTime ;
    skos:altLabel "dictionary"@en ;
    skos:broader <https://vocabs.acdh.oeaw.ac.at/dha-taxonomy#concept23> ;
    skos:definition "a structured list of words or multi-word expressions providing reference information about their meaning, translations in other languages, pronunciation, origin, usage etc."@en ;
    skos:exactMatch <http://dbpedia.org/resource/Dictionary> ;
    skos:inScheme <https://vocabs.acdh.oeaw.ac.at/dha-taxonomy> ;
    skos:notation "lexical-resource" ;
    skos:prefLabel "lexikalische Ressource"@de,
        "lexical resource"@en .

<https://vocabs.acdh.oeaw.ac.at/dha-taxonomy#concept3> a skos:Concept ;
    dc:source "Wikipedia contributors, \"FOAF (ontology),\" Wikipedia, The Free Encyclopedia, https://en.wikipedia.org/w/index.php?title=FOAF_(ontology)&oldid=703222322 (accessed February 28, 2016)."@en ;
    dct:created "2019-03-21T17:09:50.706869+00:00"^^xsd:dateTime ;
    dct:modified "2019-05-06T12:29:08.864561+00:00"^^xsd:dateTime ;
    skos:altLabel "Friend Of A Friend"@en ;
    skos:broader <https://vocabs.acdh.oeaw.ac.at/dha-taxonomy#concept1> ;
    skos:definition "a machine-readable ontology describing persons, their activities and their relations to other people and objects"@en ;
    skos:inScheme <https://vocabs.acdh.oeaw.ac.at/dha-taxonomy> ;
    skos:notation "foaf" ;
    skos:prefLabel "FOAF"@de,
        "FOAF"@en ;
    skos:related <http://dbpedia.org/resource/FOAF> .

<https://vocabs.acdh.oeaw.ac.at/dha-taxonomy#concept30> a skos:Concept ;
    dc:source "ACDH-OEAW Team"@en ;
    dct:created "2019-04-12T15:55:18.249659+00:00"^^xsd:dateTime ;
    dct:modified "2019-05-06T12:27:28.031303+00:00"^^xsd:dateTime ;
    skos:broader <https://vocabs.acdh.oeaw.ac.at/dha-taxonomy#concept23> ;
    skos:definition "collections of texts (or just sentences) annotated with complete syntactic structure"@en ;
    skos:inScheme <https://vocabs.acdh.oeaw.ac.at/dha-taxonomy> ;
    skos:notation "treebank" ;
    skos:prefLabel "Treebank"@de,
        "treebank"@en ;
    skos:related <http://dbpedia.org/resource/Treebank> .

<https://vocabs.acdh.oeaw.ac.at/dha-taxonomy#concept32> a skos:Concept ;
    dc:source "Maarten Van Gompel, \"FoLiA Format for Linguistic Annotation.\" FoLiA. Accessed June 13, 2016. https://proycon.github.io/folia/."@en ;
    dct:created "2019-04-12T15:59:00.898896+00:00"^^xsd:dateTime ;
    dct:modified "2019-05-06T12:30:04.575256+00:00"^^xsd:dateTime ;
    skos:altLabel "Format for Linguistic Annotation"@en ;
    skos:broader <https://vocabs.acdh.oeaw.ac.at/dha-taxonomy#concept31> ;
    skos:definition "an XML-based annotation format, suitable for the representation of linguistically annotated language resources"@en ;
    skos:inScheme <https://vocabs.acdh.oeaw.ac.at/dha-taxonomy> ;
    skos:notation "folia" ;
    skos:prefLabel "Folia"@de,
        "Folia"@en .

<https://vocabs.acdh.oeaw.ac.at/dha-taxonomy#concept34> a skos:Concept ;
    dc:source "Wikipedia contributors, \"Entity linking,\" Wikipedia, The Free Encyclopedia, https://en.wikipedia.org/w/index.php?title=Entity_linking&oldid=833222865 (accessed April 3, 2018)."@en ;
    dct:created "2019-04-12T16:02:18.490401+00:00"^^xsd:dateTime ;
    dct:modified "2019-05-06T12:27:59.661352+00:00"^^xsd:dateTime ;
    skos:altLabel "Named Entity Linking"@en ;
    skos:broader <https://vocabs.acdh.oeaw.ac.at/dha-taxonomy#concept33> ;
    skos:inScheme <https://vocabs.acdh.oeaw.ac.at/dha-taxonomy> ;
    skos:notation "entity-linking" ;
    skos:note "the task of determining the identity of entities mentioned in the text that requires a knowledge base containing the entities to which entity mentions can be linked"@en ;
    skos:prefLabel "Entity-Verknüpfung"@de,
        "entity linking"@en .

<https://vocabs.acdh.oeaw.ac.at/dha-taxonomy#concept35> a skos:Concept ;
    dc:source "based on: Wikipedia contributors, \"Lemmatisation,\" Wikipedia, The Free Encyclopedia, https://en.wikipedia.org/w/index.php?title=Lemmatisation&oldid=692695396 (accessed February 28, 2016)."@en ;
    dct:created "2019-04-12T16:02:55.921954+00:00"^^xsd:dateTime ;
    dct:modified "2019-05-06T12:28:14.656304+00:00"^^xsd:dateTime ;
    skos:broader <https://vocabs.acdh.oeaw.ac.at/dha-taxonomy#concept33> ;
    skos:definition "a process of grouping together the different inflected forms of a word to its canonical form so that they can be analysed as a single item"@en ;
    skos:inScheme <https://vocabs.acdh.oeaw.ac.at/dha-taxonomy> ;
    skos:notation "lemmatisation" ;
    skos:prefLabel "Lemmatisierung"@de,
        "lemmatisation"@en .

<https://vocabs.acdh.oeaw.ac.at/dha-taxonomy#concept36> a skos:Concept ;
    dc:creator "ACDH-OEAW Team" ;
    dct:created "2019-04-12T16:04:39.932181+00:00"^^xsd:dateTime ;
    dct:modified "2019-05-06T12:28:26.769337+00:00"^^xsd:dateTime ;
    skos:altLabel "Named Entity Recognition"@en ;
    skos:broader <https://vocabs.acdh.oeaw.ac.at/dha-taxonomy#concept33> ;
    skos:definition "a process of identifying mentions of individuals/entities in a text"@en ;
    skos:inScheme <https://vocabs.acdh.oeaw.ac.at/dha-taxonomy> ;
    skos:notation "ner" ;
    skos:prefLabel "NER"@de,
        "NER"@en .

<https://vocabs.acdh.oeaw.ac.at/dha-taxonomy#concept4> a skos:Concept ;
    dc:source "based on Wikipedia contributors, \"Resource Description Framework,\" Wikipedia, The Free Encyclopedia, https://en.wikipedia.org/w/index.php?title=Resource_Description_Framework&oldid=722184246 (accessed June 13, 2016)."@en ;
    dct:created "2019-03-21T17:10:42.661494+00:00"^^xsd:dateTime ;
    dct:modified "2019-05-06T12:29:20.776902+00:00"^^xsd:dateTime ;
    skos:altLabel "RDF"@de,
        "Resource Description Framework"@en ;
    skos:broader <https://vocabs.acdh.oeaw.ac.at/dha-taxonomy#concept1> ;
    skos:definition "a group of W3C specifications designed as a metadata data model to provide interoperability between applications that exchange machine-understandable information on the Web. It is used as a general method for conceptual description or modeling of information."@en ;
    skos:inScheme <https://vocabs.acdh.oeaw.ac.at/dha-taxonomy> ;
    skos:notation "rdf" ;
    skos:prefLabel "RDF"@en ;
    skos:related <http://d-nb.info/gnd/4737512-7> .

<https://vocabs.acdh.oeaw.ac.at/dha-taxonomy#concept5> a skos:Concept ;
    dc:source "based on Wikipedia contributors, \"Simple Knowledge Organization System,\" Wikipedia, The Free Encyclopedia, https://en.wikipedia.org/w/index.php?title=Simple_Knowledge_Organization_System&oldid=703222387 (accessed February 28, 2016)."@en ;
    dct:created "2019-03-21T17:11:45.666812+00:00"^^xsd:dateTime ;
    dct:modified "2019-05-06T12:29:33.049427+00:00"^^xsd:dateTime ;
    skos:altLabel "Simple Knowledge Organisation System"@en ;
    skos:broader <https://vocabs.acdh.oeaw.ac.at/dha-taxonomy#concept1> ;
    skos:definition "a W3C recommendation format designed for the representation of thesauri, classification schemes, taxonomies, subject-heading systems, or any other type of structured controlled vocabulary"@en ;
    skos:inScheme <https://vocabs.acdh.oeaw.ac.at/dha-taxonomy> ;
    skos:notation "skos" ;
    skos:prefLabel "SKOS"@de,
        "SKOS"@en .

<https://vocabs.acdh.oeaw.ac.at/dha-taxonomy#concept31> a skos:Concept ;
    dc:creator "ACDH-OEAW Team" ;
    dct:created "2019-04-12T15:56:50.259954+00:00"^^xsd:dateTime ;
    dct:modified "2019-05-06T12:29:53.905655+00:00"^^xsd:dateTime ;
    skos:definition "the representation of printed texts in digital format"@en ;
    skos:inScheme <https://vocabs.acdh.oeaw.ac.at/dha-taxonomy> ;
    skos:narrower <https://vocabs.acdh.oeaw.ac.at/dha-taxonomy#concept17>,
        <https://vocabs.acdh.oeaw.ac.at/dha-taxonomy#concept32> ;
    skos:notation "text-encoding" ;
    skos:prefLabel "text encoding"@de,
        "text encoding"@en ;
    skos:topConceptOf <https://vocabs.acdh.oeaw.ac.at/dha-taxonomy> .

<https://vocabs.acdh.oeaw.ac.at/dha-taxonomy#concept33> a skos:Concept ;
    dc:creator "ACDH-OEAW Team" ;
    dct:created "2019-04-12T16:01:03.094918+00:00"^^xsd:dateTime ;
    dct:modified "2019-05-06T12:27:42.225179+00:00"^^xsd:dateTime ;
    skos:altLabel "Natural Language Processing"@en ;
    skos:definition "tools and methods to process (analyse, enrich, transform) language resources"@en ;
    skos:inScheme <https://vocabs.acdh.oeaw.ac.at/dha-taxonomy> ;
    skos:narrower <https://vocabs.acdh.oeaw.ac.at/dha-taxonomy#concept34>,
        <https://vocabs.acdh.oeaw.ac.at/dha-taxonomy#concept35>,
        <https://vocabs.acdh.oeaw.ac.at/dha-taxonomy#concept36> ;
    skos:notation "nlp" ;
    skos:prefLabel "NLP"@de,
        "NLP"@en ;
    skos:related <http://dbpedia.org/resource/Natural_language_processing> ;
    skos:topConceptOf <https://vocabs.acdh.oeaw.ac.at/dha-taxonomy> .

<https://vocabs.acdh.oeaw.ac.at/dha-taxonomy#concept1> a skos:Concept ;
    dc:creator "ACDH" ;
    dc:source "based on \"Vocabularies.\" W3C. Accessed June 13, 2016. https://www.w3.org/standards/semanticweb/ontology."@en ;
    dct:created "2019-03-15T15:19:06.273650+00:00"^^xsd:dateTime ;
    dct:modified "2019-05-06T12:28:46.975509+00:00"^^xsd:dateTime ;
    skos:definition "machine-readable terminologies that define concepts and relationships used to describe and organize data on the web"@en ;
    skos:inScheme <https://vocabs.acdh.oeaw.ac.at/dha-taxonomy> ;
    skos:narrower <https://vocabs.acdh.oeaw.ac.at/dha-taxonomy#concept2>,
        <https://vocabs.acdh.oeaw.ac.at/dha-taxonomy#concept3>,
        <https://vocabs.acdh.oeaw.ac.at/dha-taxonomy#concept4>,
        <https://vocabs.acdh.oeaw.ac.at/dha-taxonomy#concept5> ;
    skos:notation "language-resource" ;
    skos:prefLabel "semantische Web vokabulare"@de,
        "semantic web vocabularies"@en ;
    skos:related <http://dbpedia.org/resource/Semantic_Web> ;
    skos:topConceptOf <https://vocabs.acdh.oeaw.ac.at/dha-taxonomy> .

<https://vocabs.acdh.oeaw.ac.at/dha-taxonomy#concept23> a skos:Concept ;
    dc:source "Simons, G. F., and Bird, S. “Toward a Global Infrastructure for the Sustainability of Language Resources.” Proceedings of 22nd Pacific Asia Conference on Language, Information and Computation, 20–22 November 2008, Cebu City, Philippines. Accessed March 30, 2016. http://www-01.sil.org/~simonsg/preprint/PACLIC22.pdf."@en ;
    dct:created "2019-04-12T13:18:49.838435+00:00"^^xsd:dateTime ;
    dct:modified "2019-05-06T12:25:59.634029+00:00"^^xsd:dateTime ;
    skos:definition "a language resource is any physical or digital item that is a product of language documentation, description, or development or is a tool that specifically supports the creation and use of such products"@en ;
    skos:inScheme <https://vocabs.acdh.oeaw.ac.at/dha-taxonomy> ;
    skos:narrower <https://vocabs.acdh.oeaw.ac.at/dha-taxonomy#concept26>,
        <https://vocabs.acdh.oeaw.ac.at/dha-taxonomy#concept27>,
        <https://vocabs.acdh.oeaw.ac.at/dha-taxonomy#concept28>,
        <https://vocabs.acdh.oeaw.ac.at/dha-taxonomy#concept29>,
        <https://vocabs.acdh.oeaw.ac.at/dha-taxonomy#concept30> ;
    skos:notation "historical-resource" ;
    skos:prefLabel "Sprachressource"@en,
        "language resource"@en ;
    skos:related <http://d-nb.info/gnd/16113632-1> ;
    skos:topConceptOf <https://vocabs.acdh.oeaw.ac.at/dha-taxonomy> .

<https://vocabs.acdh.oeaw.ac.at/dha-taxonomy> a skos:ConceptScheme ;
    rdfs:label "DHA Taxonomy"@en ;
    dc:contributor "DHA consortium" ;
    dc:creator "ACDH-OEAW Team" ;
    dc:description "DHA taxonomy is a knowledge organization system designed to describe subjects, resources and tools within activities of Digital Humanities Austria."@en ;
    dc:language "English" ;
    dc:publisher "ACDH-OEAW" ;
    dc:relation <http://www.digital-humanities.at/en> ;
    dc:subject "Computational methods in humanities",
        "Cultural analytics",
        "Text technologies" ;
    dc:title "DHA Taxonomie"@de,
        "DHA Taxonomy"@en ;
    dct:created "2019-03-15T15:17:40.943281+00:00"^^xsd:dateTime ;
    dct:issued "2018-04-03"^^xsd:dateTime ;
    dct:license "https://creativecommons.org/licenses/by/4.0/" ;
    dct:modified "2019-06-13T14:56:21.502226+00:00"^^xsd:dateTime ;
    dct:rightsHolder "ACDH-OEAW" ;
    owl:versionInfo "1.0" ;
    skos:hasTopConcept <https://vocabs.acdh.oeaw.ac.at/dha-taxonomy#concept1>,
        <https://vocabs.acdh.oeaw.ac.at/dha-taxonomy#concept20>,
        <https://vocabs.acdh.oeaw.ac.at/dha-taxonomy#concept21>,
        <https://vocabs.acdh.oeaw.ac.at/dha-taxonomy#concept23>,
        <https://vocabs.acdh.oeaw.ac.at/dha-taxonomy#concept24>,
        <https://vocabs.acdh.oeaw.ac.at/dha-taxonomy#concept25>,
        <https://vocabs.acdh.oeaw.ac.at/dha-taxonomy#concept31>,
        <https://vocabs.acdh.oeaw.ac.at/dha-taxonomy#concept33> .

